callback spec and proof using ints

src/Lib/VstCallback.v
@@ -2,6 +2,7 @@ Require Import Core.Core Core.Tactics.
 Require Import VST.floyd.proofauto.
 Require Import VST.floyd.library.
 Require Import Clight.asn_application Lib.Stdlib.
+Require Import Core.Notations.
 
 Definition Vprog : varspecs. mk_varspecs prog. Defined.
 Instance CompSpecs : compspecs. make_compspecs prog. Defined.
@@ -36,7 +37,7 @@ Definition callback  : funspec :=
                    (mk_enc_key (Vptr buf_b buf_ofs) buf_size computed_size) 
                    key_p;
           if buf_size <? computed_size + size 
-          then memory_block Tsh buf_size (Vptr buf_b buf_ofs)
+          then emp
           else memory_block Tsh size (Vptr buf_b (Ptrofs.add buf_ofs
                                       (Ptrofs.repr computed_size))))    
      POST [tint]
@@ -44,8 +45,7 @@ Definition callback  : funspec :=
       LOCAL (temp ret_temp Vzero)
       SEP (data_at Tsh (tarray tuchar (Zlength data)) (map Vint data) data_p;
            if buf_size <? computed_size + size 
-           then memory_block Tsh buf_size (Vptr buf_b buf_ofs) *
-                data_at Tsh enc_key_s 
+           then data_at Tsh enc_key_s 
                    (mk_enc_key (Vptr buf_b buf_ofs) 0 (computed_size + size))  
                    key_p
            else 
@@ -55,6 +55,91 @@ Definition callback  : funspec :=
               data_at Tsh enc_key_s 
                       (mk_enc_key (Vptr buf_b buf_ofs)
                                   buf_size (computed_size + size)) key_p)). 
+
+Definition callback_int  : funspec :=
+    WITH data : list int, data_p : val, 
+         size : int,
+         key : val, key_p : val, 
+         buf_b : block, buf_ofs : ptrofs,
+         buf_size : int, computed_size : int
+    PRE [tptr tvoid, tuint, tptr tvoid]
+      PROP ()
+      PARAMS (data_p; Vint size; key_p)
+      GLOBALS ()
+      SEP 
+      (data_at Tsh (tarray tuchar (Int.unsigned size)) (map Vint data) data_p;
+       data_at Tsh enc_key_s 
+               (Vptr buf_b buf_ofs, (Vint buf_size, Vint computed_size)) key_p;
+       if (buf_size <u computed_size + size)%int 
+       then emp
+       else memory_block Tsh (Int.unsigned size)
+                         (Vptr buf_b (Ptrofs.add buf_ofs (Ptrofs.of_int computed_size))))    
+     POST [tint]
+      PROP ()
+      LOCAL (temp ret_temp Vzero)
+      SEP (data_at Tsh (tarray tuchar (Int.unsigned size)) (map Vint data) data_p;
+           if (buf_size <u computed_size + size)%int 
+           then data_at Tsh enc_key_s 
+                   (Vptr buf_b buf_ofs, (Vzero, Vint (computed_size + size))%int)  
+                   key_p
+           else 
+             (data_at Tsh (tarray tuchar (Int.unsigned size)) (map Vint data) 
+                      (Vptr buf_b (Ptrofs.add
+                                     buf_ofs
+                                     (Ptrofs.of_int computed_size))) *
+              data_at Tsh enc_key_s ((Vptr buf_b buf_ofs), 
+                                     (Vint buf_size, 
+                                     Vint (computed_size + size)%int)) key_p)). 
+
+Definition callback_overrun_spec_int : ident * funspec :=
+  DECLARE _overrun_encoder_cb callback_int.
+
+Definition Gprog := ltac:(with_library prog [callback_overrun_spec_int; (_memcpy, memcpy_spec)]).
+
+Theorem bool_der_encode_int : semax_body Vprog Gprog f_overrun_encoder_cb 
+                                     callback_overrun_spec_int.
+  Proof.
+    start_function.
+    destruct (buf_size <u computed_size + size)%int eqn : Q.
+    - 
+    repeat forward.
+    forward_if 
+      (PROP ()
+       LOCAL (temp _t'3 (Vint buf_size); 
+              temp _t'2 (Vint computed_size);
+              temp _key key_p; temp _data data_p; 
+              temp _size (Vint size);
+              temp _keyp key_p)
+       SEP (data_at Tsh (tarray tuchar (Int.unsigned size)) (map Vint data) data_p;
+            data_at Tsh enc_key_s (Vptr buf_b buf_ofs, (Vzero, Vint computed_size)) 
+                   key_p));
+    repeat (forward || entailer! || congruence).  
+    - 
+    repeat forward.
+    forward_if
+      (PROP ()
+       LOCAL (
+         temp _t'5 (Vint computed_size); 
+         temp _t'4 (Vptr buf_b buf_ofs);
+         temp _t'3 (Vint buf_size); 
+         temp _t'2 (Vint computed_size);
+         temp _key key_p; temp _data data_p; 
+         temp _size (Vint size);
+         temp _keyp key_p)
+       SEP (data_at Tsh (tarray tuchar (Int.unsigned size)) (map Vint data) data_p;
+            data_at Tsh (tarray tuchar (Int.unsigned size)) (map Vint data) 
+                      (Vptr buf_b (Ptrofs.add buf_ofs
+                                              (Ptrofs.of_int computed_size)));
+            data_at Tsh enc_key_s (Vptr buf_b buf_ofs,
+                                   (Vint buf_size, Vint (computed_size))) key_p));
+       repeat (forward || entailer! || congruence).
+    assert (Int.repr (Int.unsigned size) = size) as II by auto with ints.
+    forward_call (Tsh, Tsh, Vptr buf_b 
+                 (Ptrofs.add buf_ofs (Ptrofs.of_int computed_size)), data_p,
+                 (Int.unsigned size), data);  
+      auto with ints; 
+      try rewrite II; entailer!.
+Qed.
 
 Definition dummy_callback  : funspec :=
     WITH  data_p : val, size : Z,
@@ -72,9 +157,9 @@ Definition dummy_callback  : funspec :=
 Definition callback_overrun_spec : ident * funspec :=
   DECLARE _overrun_encoder_cb callback.
 
-Definition Gprog := ltac:(with_library prog [callback_overrun_spec; (_memcpy, memcpy_spec)]).
+Definition Gprog2 := ltac:(with_library prog [callback_overrun_spec; (_memcpy, memcpy_spec)]).
 
-Theorem bool_der_encode : semax_body Vprog Gprog f_overrun_encoder_cb 
+Theorem bool_der_encode : semax_body Vprog Gprog2 f_overrun_encoder_cb 
                                      callback_overrun_spec.
   Proof.
     start_function.
@@ -90,7 +175,6 @@ Theorem bool_der_encode : semax_body Vprog Gprog f_overrun_encoder_cb
               temp _size (Vint (Int.repr size));
               temp _keyp key_p)
        SEP (data_at Tsh (tarray tuchar (Zlength data)) (map Vint data) data_p;
-            memory_block Tsh buf_size (Vptr buf_b buf_ofs) ;
             data_at Tsh enc_key_s 
                    (mk_enc_key (Vptr buf_b buf_ofs) 0 computed_size) 
                    key_p));
